fr.inria.atlanmod.coqtl.coq/core/Model.v
@@ -5,17 +5,13 @@ Scheme Equality for list.
 (** * Model
   Each model is constructed by a list of {@code ModelElement} and {@ModelLink}. **)
 
-Class Model (ModelElement: Type) (ModelLink: Type) :=
+Class Model (ModelElement: Type) :=
   {
     modelElements : list ModelElement;
-    modelLinks : list ModelLink;
   }.
 
-Definition allModelElements {ModelElement: Type} {ModelLink: Type} (m: Model ModelElement ModelLink) : list ModelElement :=
-  (@modelElements _ _ m).
-
-Definition allModelLinks {ModelElement: Type} {ModelLink: Type} (m: Model ModelElement ModelLink) : list ModelLink :=
-  (@modelLinks _ _ m).
+Definition allModelElements {ModelElement: Type} (m: Model ModelElement) : list ModelElement :=
+  (@modelElements _ m).
 
 (*
  allModelElements and allModelLinks are fields of record Model.
@@ -23,6 +19,5 @@ Definition allModelLinks {ModelElement: Type} {ModelLink: Type} (m: Model ModelE
  @allModelElements _ _ a.
  *)
 
-Definition Model_beq {ME ML: Type} (ME_beq: ME -> ME -> bool) (ML_beq: ML -> ML -> bool) (m1 m2: Model ME ML) :=
-  andb (list_beq ME_beq (@modelElements _ _ m1) (@modelElements _ _ m2))
-  (list_beq ML_beq (@modelLinks _ _ m1) (@modelLinks _ _ m2)).
+Definition Model_beq {ME: Type} (ME_beq: ME -> ME -> bool) (m1 m2: Model ME) :=
+  (list_beq ME_beq (@modelElements _ m1) (@modelElements _ m2)).
