fr.inria.atlanmod.coqtl.coq/core/modeling/twophases/TwoPhaseCertification.v
@@ -69,7 +69,7 @@ Proof.
 Qed. 
 
 Lemma tr_executeTraces_in_links :
-forall (tr: Transformation) (sm : SourceModel) (tl : TargetModelLink),
+forall (tr: Transformation) (sm : SourceModel) (tl : TargetModelElement),
       In tl (allModelLinks (executeTraces tr sm)) <->
           (exists (sp : list SourceModelElement),
           In sp (allTuples tr sm) /\
@@ -168,7 +168,7 @@ Qed.
 (** * Apply **)
 
 Lemma tr_applyTraces_in :
-forall (tr: Transformation) (sm : SourceModel) (sp: list SourceModelElement) (tl : TargetModelLink) (tls: list TraceLink),
+forall (tr: Transformation) (sm : SourceModel) (sp: list SourceModelElement) (tl : TargetModelElement) (tls: list TraceLink),
   In tl (applyTraces tr sm tls) <->
   (exists (sp : list SourceModelElement),
       In sp (allTuples tr sm) /\
@@ -179,7 +179,7 @@ Proof.
 Qed.
 
 Lemma tr_applyPatternTraces_in:
-forall (tr: Transformation) (sm : SourceModel) (sp: list SourceModelElement) (tl : TargetModelLink) (tls: list TraceLink),
+forall (tr: Transformation) (sm : SourceModel) (sp: list SourceModelElement) (tl : TargetModelElement) (tls: list TraceLink),
   In tl (applyPatternTraces tr sm sp tls) <->
   (exists (r : Rule),
           In r (matchPattern tr sm sp) /\
@@ -190,7 +190,7 @@ Proof.
 Qed.
 
 Lemma tr_applyRuleOnPatternTraces_in : 
-forall (tr: Transformation) (r : Rule) (sm : SourceModel) (sp: list SourceModelElement) (tl : TargetModelLink) (tls: list TraceLink),
+forall (tr: Transformation) (r : Rule) (sm : SourceModel) (sp: list SourceModelElement) (tl : TargetModelElement) (tls: list TraceLink),
     In tl (applyRuleOnPatternTraces r tr sm sp tls) <->
     (exists (i: nat),
         In i (seq 0 (evalIteratorExpr r sm sp)) /\
@@ -201,7 +201,7 @@ Proof.
 Qed.
 
 Lemma tr_applyIterationOnPatternTraces_in : 
-    forall (tr: Transformation) (r : Rule) (sm : SourceModel) (sp: list SourceModelElement) (tl : TargetModelLink) (i:nat)  (tls: list TraceLink),
+    forall (tr: Transformation) (r : Rule) (sm : SourceModel) (sp: list SourceModelElement) (tl : TargetModelElement) (i:nat)  (tls: list TraceLink),
       In tl (applyIterationOnPatternTraces r tr sm sp i tls) <->
       (exists (ope: OutputPatternElement),
           In ope (Rule_getOutputPatternElements r) /\ 
@@ -212,7 +212,7 @@ Proof.
 Qed.
 
 Lemma tr_applyElementOnPatternTraces_in : 
-    forall (tr: Transformation) (sm : SourceModel) (sp: list SourceModelElement) (tl : TargetModelLink) 
+    forall (tr: Transformation) (sm : SourceModel) (sp: list SourceModelElement) (tl : TargetModelElement) 
             (i:nat) (ope: OutputPatternElement)  (tls: list TraceLink),
       In tl (applyElementOnPatternTraces ope tr sm sp i tls) <->
       (exists (oper: OutputPatternLink) (te: TargetModelElement),
@@ -311,7 +311,7 @@ Proof.
 Qed.
 
 Lemma tr_execute_in_links' :
-forall (tr: Transformation) (sm : SourceModel) (tl : TargetModelLink),
+forall (tr: Transformation) (sm : SourceModel) (tl : TargetModelElement),
   In tl (allModelLinks (executeTraces tr sm)) <->
   (exists (sp : list SourceModelElement),
       In sp (allTuples tr sm) /\
@@ -325,7 +325,7 @@ Proof.
 Qed.
 
 (*Instance TwoPhaseCoqTLEngine :
-TransformationEngineModeling (@ModelingCoqTLEngine SourceModelElement SourceModelLink TargetModelElement TargetModelLink):=
+TransformationEngineModeling (@ModelingCoqTLEngine SourceModelElement SourceModelLink TargetModelElement TargetModelElement):=
 {
   SourceModelClass := SourceModelClass;
   SourceModelReference := SourceModelReference;
@@ -350,7 +350,7 @@ Instance CoqTLEngine :
     SourceModelReference := SourceModelReference;
     TargetModelElement := TargetModelElement;
     TargetModelClass := TargetModelClass;
-    TargetModelLink := TargetModelLink;
+    TargetModelElement := TargetModelElement;
     TargetModelReference := TargetModelReference;
 
     (* syntax and accessors *)
